\documentclass{beamer}

\usepackage{mathpartir}
\usepackage{hyperref}
\usepackage{mathtools}
\usepackage{listings}
\usepackage[utf8]{inputenc}


\lstset{
    identifierstyle=\color{black},
    % textcolor=blue,
    % keywordstyle=\color{blue},
    keywordstyle=\text,
    basicstyle=\ttfamily,
    mathescape=true,
    showspaces=false,
    morekeywords={let, fix}
}

\title{Subtyping Constraints and Type Inference}
\author{Thomas Logan}
% \date{18 November 2022}

\begin{document}

\begin{frame}
  \titlepage
\end{frame}

\begin{frame}
  \frametitle{When Subtyping Constraints Liberate}

  \begin{itemize}
  \item LIONEL PARREAUX, HKUST, Hong Kong, China
  \item ALEKSANDER BORUCH-GRUSZECKI, EPFL, Switzerland
  \item ANDONG FAN, HKUST, Hong Kong, China
  \item CHUN YIN CHAU, HKUST, Hong Kong, China
  \end{itemize}
\end{frame}

\begin{frame}[fragile]
  \frametitle{Impoverished Type Inference}

  \begin{lstlisting}
foo f = (f 123, f True)
  \end{lstlisting}

\end{frame}


\begin{frame}[fragile]
  \frametitle{Satifcatory Typing 1}

  \begin{itemize}
  \item should allow
  \begin{lstlisting}
foo (fun x => x)
  \end{lstlisting}
  \item where
  \begin{lstlisting}
(fun x => x) : ALL a . a -> a
  \end{lstlisting}
  \end{itemize}

\end{frame}


\begin{frame}[fragile]
  \frametitle{Satifcatory Typing 2}

  \begin{itemize}
  \item should allow
  \begin{lstlisting}
foo (fun x => some x)
  \end{lstlisting}
  \item where
  \begin{lstlisting}
(fun x => some x) : ALL a . a -> Option a
  \end{lstlisting}
  \end{itemize}

\end{frame}

\begin{frame}[fragile]
  \frametitle{Intersection as Savior}

  \begin{lstlisting}
foo f = (f 123, f True)
  \end{lstlisting}

  \begin{lstlisting}
foo : ALL a b . 
      ((Int -> a) & (Bool -> b)) -> (a,b)
  \end{lstlisting}
\end{frame}


\begin{frame}[fragile]
  \frametitle{Instantiation as Subtyping}

  \begin{itemize}
  \item application 
  \begin{lstlisting}
foo (fun x => some x)
  \end{lstlisting}
  \item generates subtyping constraint to be checked or solved 
  \begin{lstlisting}
(ALL a . a -> Option a) 
         <: 
((Int -> c) & (Bool -> d))
  \end{lstlisting}
  \end{itemize}
\end{frame}


\begin{frame}[fragile]
  \frametitle{Intersection as Constrained Parametric Polymorphism}
  \begin{itemize}
  \item intersection in parameter type 
  \begin{lstlisting}
ALL a b . 
  ((Int -> a) & (Bool -> b)) -> (a,b)
  \end{lstlisting}
  \item is the weakest interpretation of the parameter type in 
  \begin{lstlisting}
ALL a b c 
  {c <: Int -> a, c <: Bool -> b}. 
  c -> (a,b)
  \end{lstlisting}
  \end{itemize}
\end{frame}





%%%%%%%%%%%%%%%%%%%%%%%%%%%%%%%%%%%%%%%%

\begin{frame}[fragile]
  \frametitle{}

  \begin{lstlisting}[language=Python]
  def foo(x):
      if isinstance(x, int):
          return x + 1 
      else:
        return x + "abc"
  \end{lstlisting}
\end{frame}

\begin{frame}[fragile]
  \frametitle{Prescribed static bounds with datatypes}

  \begin{lstlisting}[language=ML]
  datatype int_or_str = 
      Int of int | 
      Str of string

  fun foo(Int x) = x + 1
    | foo(Str x) = x . "abc"
  \end{lstlisting}

\end{frame}

\begin{frame}[fragile]
  \frametitle{Specification}
  \begin{itemize}
  \item Types as specification 
    \begin{itemize}
    \item Universal spec: examples, abstract values, resource usage, 
      pure, temporal, quantitative, probabilistic 
    \end{itemize}
  \item Propagation of types   
    \begin{itemize}
    \item Expected types decomposed to locally guide at holes and leaf terms   
    \item Actual types synthesized in case annotations missing 
    \end{itemize}

  \item Expressivity of types    
    \begin{itemize}
    \item Subtyping since static bounds are unprescribed 
    \item Unification; solving for unknown types in composition 
    \item Unions and intersections to widen and narrow static bounds 
    \item Precise relations to guide effectively   
    \end{itemize}
  \end{itemize}
\end{frame}

\begin{frame}[fragile]
  \frametitle{Propagation: down}

  \begin{lstlisting}
  $\lambda$ n : nat $\Rightarrow$
    let first = ($\lambda$ (x,y) : (str $\times$ str) $\Rightarrow$ x) .
    first (n, _) 
  \end{lstlisting}

\end{frame}

\begin{frame}[fragile]
  \frametitle{Propagation: down}

  \begin{lstlisting}
  $\lambda$ n : nat $\Rightarrow$
    let first = ($\lambda$ (x,y) : (str $\times$ str) $\Rightarrow$ x) .
    first (n, _) 

    
  (n, _) : str $\times$ str
  n : str   
  nat $\leq$ str 
  _ : str  
  \end{lstlisting}

\end{frame}

\begin{frame}[fragile]
  \frametitle{Propagation: up}

  \begin{lstlisting}
  $\lambda$ upper : str $\rightarrow$ str $\Rightarrow$
  $\hdots$
  $\lambda$ x $\Rightarrow$ $\lambda$ y $\Rightarrow$
    cons*(upper x, cons*(upper y,nil*()))
  \end{lstlisting}

\end{frame}

\begin{frame}[fragile]
  \frametitle{Propagation: up}

  \begin{lstlisting}

  $\lambda$ upper : str $\rightarrow$ str $\Rightarrow$
  $\hdots$
  $\lambda$ x $\Rightarrow$ $\lambda$ y $\Rightarrow$
    cons*(upper x,cons*(upper y,nil*()))


  str $\rightarrow$ str $\rightarrow$
    cons.(str $\times$ cons.(str $\times$ nil.$\diamondsuit$))
  \end{lstlisting}

\end{frame}

\begin{frame}[fragile]
  \frametitle{Expressivity: widening}

  \begin{lstlisting}
  ($\lambda$ pair : $\forall$ $\alpha$ $\Rightarrow$ $\alpha$ $\rightarrow$ $\alpha$ $\rightarrow$ ($\alpha$ $\times$ $\alpha$) $\Rightarrow$ 
  ($\lambda$ n : int $\Rightarrow$ ($\lambda$ s : str $\Rightarrow$ 
    let p = pair n s
    $\hdots$
  )))

  \end{lstlisting}
\end{frame}


\begin{frame}[fragile]
  \frametitle{Expressivity: widening}

  \begin{lstlisting}
  ($\lambda$ pair : $\forall$ $\alpha$ $\Rightarrow$ $\alpha$ $\rightarrow$ $\alpha$ $\rightarrow$ ($\alpha$ $\times$ $\alpha$) $\Rightarrow$ 
  ($\lambda$ n : int $\Rightarrow$ ($\lambda$ s : str $\Rightarrow$ 
    let p = pair n s
    $\hdots$
  )))

  $\alpha$ $\mapsto$ (int | ?) 
  $\alpha$ $\mapsto$ (int | str | ?)
  pair : $\top$ $\rightarrow$ $\top$ $\rightarrow$ (int | str) $\times$ (int | str)

  \end{lstlisting}
\end{frame}


\begin{frame}[fragile]
  \frametitle{Expressivity: narrowing}

  \begin{lstlisting}
  ($\lambda$ i2n : int $\rightarrow$ nat $\Rightarrow$ 
  ($\lambda$ s2n : str $\rightarrow$ nat $\Rightarrow$ 
    let f = $\lambda$ x $\Rightarrow$ (i2n x, s2n x)
    $\hdots$
  ))
  \end{lstlisting}
\end{frame}

\begin{frame}[fragile]
  \frametitle{Expressivity: narrowing}

  \begin{lstlisting}
  ($\lambda$ i2n : int $\rightarrow$ nat $\Rightarrow$ 
  ($\lambda$ s2n : str $\rightarrow$ nat $\Rightarrow$ 
    let f = $\lambda$ x $\Rightarrow$ (i2n x, s2n x)
    $\hdots$
  ))
  
  x : $\alpha$
  $\alpha$ $\mapsto$ (int ; ?)
  $\alpha$ $\mapsto$ (int ; str ; ?)
  x : $\bot$
  $\lambda$ x $\Rightarrow$ (i2n x, s2n x) : 
    (int ; str) $\rightarrow$ (nat $\times$ nat) 
  \end{lstlisting}
\end{frame}

\begin{frame}[fragile]
  \frametitle{Expressivity: relational record}

  \begin{lstlisting}[]
  let measurement : $\mu$ (nat $\times$ list) $\Rightarrow$ 
    zero.$\diamondsuit$ $\times$ nil.$\diamondsuit$ | 
    succ.nat $\times$ cons.(? $\times$ list)
  \end{lstlisting} 

\end{frame}

\begin{frame}[fragile]
  \frametitle{Expressivity: relational record expanded}

  \begin{lstlisting}[]
  let measurement : 
  $\exists$ $\alpha$ $\Rightarrow$ $\mu$ nat_and_list $\Rightarrow$ 
    zero.$\diamondsuit$ $\times$ nil.$\diamondsuit$ | 
    $\exists$ nat list :: 
      (nat $\times$ list) $\leq$ nat_and_list $\Rightarrow$ 
      succ.nat.$\times$ cons.($\alpha$ $\times$ list)
  \end{lstlisting}

\end{frame}

\begin{frame}[fragile]
  \frametitle{Expressivity: relational record comparison (Synquid)}

  \begin{lstlisting}[keywords={termination, measure, data, where}]
  termination measure len :: List $\beta$ $\rightarrow$ Nat 
  data List $\beta$ where
    Nil :: {v: List $\beta$ | len v = 0}
    Cons :: $\beta$ $\rightarrow$ xs: List $\beta$ $\rightarrow$ 
      {v: List $\beta$ | len v = len xs + 1}

  \end{lstlisting}
\end{frame}

\begin{frame}[fragile]
  \frametitle{Expressivity: relational function}

  \begin{lstlisting}[]
  let replicate : 
  $\forall$ $\alpha$ $\Rightarrow$ $\alpha$ $\rightarrow$ $\nu$ (nat $\rightarrow$ list) $\Rightarrow$ 
    zero.$\diamondsuit$ $\rightarrow$ nil.$\diamondsuit$ ; 
    succ.nat $\rightarrow$ cons.($\alpha$ $\times$ list)
  \end{lstlisting}


\end{frame}

\begin{frame}[fragile]

  \frametitle{Expressivity: relational function expanded}

  \begin{lstlisting}[]
  let replicate : 
  $\forall$ $\alpha$ $\Rightarrow$ $\alpha$ $\rightarrow$ $\nu$ nat_to_list $\Rightarrow$ 
    zero.$\diamondsuit$ $\rightarrow$ nil.$\diamondsuit$ ; 
    $\forall$ nat list :: 
      nat_to_list $\leq$ (nat $\rightarrow$ list) $\Rightarrow$ 
      succ.nat $\rightarrow$ cons.($\alpha$ $\times$ list)
  \end{lstlisting}

\end{frame}

\begin{frame}[fragile]

  \frametitle{Expressivity: relational function comparison (Synquid)}

  \begin{lstlisting}[keywords={termination, measure, data, where}]
  replicate :: n:Nat $\rightarrow$ x:$\alpha$ $\rightarrow$ 
    {v: List $\alpha$ | len v = n}

  \end{lstlisting}

  \hfill
\end{frame}

\begin{frame}[fragile]
  \frametitle{Expressivity: recursive pattern matching}
  \begin{lstlisting}[]
  let replicate = 
  $\lambda$ x $\Rightarrow$ fix ($\lambda$ self $\Rightarrow$ $\lambda$ [
      zero*() $\Rightarrow$ nil*(),
      succ*n $\Rightarrow$ cons*(x, self n)
  ])

  let replicate : 
  $\forall$ $\alpha$ $\Rightarrow$ $\alpha$ $\rightarrow$ $\nu$ (nat $\rightarrow$ list) $\Rightarrow$ 
    zero.$\diamondsuit$ $\rightarrow$ nil.$\diamondsuit$ ; 
    succ.nat $\rightarrow$ cons.($\alpha$ $\times$ list)
  \end{lstlisting}
\end{frame}


\begin{frame}[fragile]
  \frametitle{Expressivity: unification with nat}

  \begin{lstlisting}[]
  nat $\equiv$ $\mu$ nat $\Rightarrow$ 
    zero.$\diamondsuit$ | 
    succ.nat


  > zero.$\diamondsuit$ $\leq$ nat 
  < $\cdot$

  > succ.succ.zero.$\diamondsuit$ $\leq$ nat 
  < $\cdot$

  > succ.$\alpha$ $\leq$ nat 
  < $\cdot$, $\alpha$ $\mapsto$ $\mu$ $\beta$ $\Rightarrow$ zero.$\diamondsuit$ | succ.$\beta$
  \end{lstlisting} 

\end{frame}

\begin{frame}[fragile]
  \frametitle{Expressivity: unification with nat and even}

  \begin{lstlisting}[]
  nat $\equiv$ $\mu$ nat $\Rightarrow$ 
    zero.$\diamondsuit$ | 
    succ.nat

  even $\equiv$ $\mu$ even $\Rightarrow$ 
    zero.$\diamondsuit$ | 
    succ.succ.even 


  > even $\leq$ nat 
  < $\cdot$

  > nat $\leq$ even 
  < $\emptyset$
  \end{lstlisting} 

\end{frame}


\begin{frame}[fragile]
  \frametitle{Expressivity: unification with nat list relation}

  \begin{lstlisting}[]
  nat_list $\equiv$ $\mu$ (nat $\times$ list) $\Rightarrow$ 
    zero.$\diamondsuit$ $\times$ nil.$\diamondsuit$ | 
    succ.nat $\times$ cons.(? $\times$ list)


  > succ.zero.$\diamondsuit$ $\times$ cons.(? $\times$ cons.(? $\times$ $\alpha$))
    $\leq$ nat_list
  < $\emptyset$

  > succ.succ.zero.$\diamondsuit$ $\times$ cons.(? $\times$ $\alpha$) 
    $\leq$ nat_list
  < $\cdot$, $\alpha$ $\mapsto$ cons.(? $\times$ nil.$\diamondsuit$)
  \end{lstlisting} 
\end{frame}


\begin{frame}[fragile]
  \frametitle{Expressivity: plus relation}

  \begin{lstlisting}[]
  $\mu$ plus $\Rightarrow$ 
    $\exists$ $\alpha$ $\Rightarrow$ 
      (x $\mapsto$ zero.$\diamondsuit$ ; y $\mapsto$ $\alpha$ ; z $\mapsto$ $\alpha$) |
    $\exists$ $\alpha$ $\beta$ $\gamma$ :: 
      (x $\mapsto$ $\alpha$ ; y $\mapsto$ $\beta$ ; z $\mapsto$ $\gamma$) $\leq$ plus $\Rightarrow$ 
      x $\mapsto$ succ.$\alpha$ ; y $\mapsto$ $\beta$ ; z $\mapsto$ succ.$\gamma$
  \end{lstlisting}
\end{frame}

\begin{frame}[fragile]
  \frametitle{Expressivity: unification with plus relation}

  \begin{lstlisting}[]
  plus $\equiv$ $\mu$ plus .
    $\exists$ $\alpha$ $\Rightarrow$ 
      (x $\mapsto$ zero.$\diamondsuit$ ; y $\mapsto$ $\alpha$ ; z $\mapsto$ $\alpha$) |
    $\exists$ $\alpha$ $\beta$ $\gamma$ :: 
      (x $\mapsto$ $\alpha$ ; y $\mapsto$ $\beta$ ; z $\mapsto$ $\gamma$) $\leq$ plus $\Rightarrow$ 
      x $\mapsto$ succ.$\alpha$ ; y $\mapsto$ $\beta$ ; z $\mapsto$ succ.$\gamma$

  > (x $\mapsto$ succ.zero.$\diamondsuit$ ; y $\mapsto$ $\alpha$ ; 
     z $\mapsto$ succ.succ.zero.$\diamondsuit$) $\leq$ plus
  < $\cdot$, $\alpha$ $\mapsto$ succ.zero.$\diamondsuit$)

  > (x $\mapsto$ $\alpha$ ; y $\mapsto$ $\beta$ ; z $\mapsto$ succ.zero.$\diamondsuit$) $\leq$ plus
  < $\cdot$, $\alpha$ $\mapsto$ zero.$\diamondsuit$, $\beta$ $\mapsto$ succ.zero.$\diamondsuit$
  < $\cdot$, $\alpha$ $\mapsto$ succ.zero $\diamondsuit$, $\beta$ $\mapsto$ zero.$\diamondsuit$
  \end{lstlisting}


\end{frame}
\begin{frame}[fragile]
  \frametitle{Expressivity: comparison to Prolog}

  \begin{lstlisting}[]
  plus(0, A, A).
  plus(s(A), B, s(C)) :- plus(A, B, C).


  $\mu$ plus .
    $\exists$ $\alpha$ $\Rightarrow$ 
      (x $\mapsto$ zero.$\diamondsuit$ ; y $\mapsto$ $\alpha$ ; z $\mapsto$ $\alpha$) |
    $\exists$ $\alpha$ $\beta$ $\gamma$ :: 
      (x $\mapsto$ $\alpha$ ; y $\mapsto$ $\beta$ ; z $\mapsto$ $\gamma$) $\leq$ plus $\Rightarrow$ 
      x $\mapsto$ succ.$\alpha$ ; y $\mapsto$ $\beta$ ; z $\mapsto$ succ.$\gamma$

  \end{lstlisting}

\end{frame}

\end{document}